src/ListUtil.v
@@ -17,3 +17,18 @@ Fixpoint nth_with_proof T (n:nat) (l:list T) (H : length(l) > n) {struct l} : T.
   refine (nth_with_proof T n l _).
   omega.
 Defined.
+
+Lemma firstn_concat : forall A (l : list A) (l' : list A), firstn (length l) (l ++ l') = l.
+  induction l; intros; simplify; equality.
+Qed.
+
+Lemma skipn_concat : forall A (l : list A) (l' : list A), skipn (length l) (l ++ l') = l'.
+  induction l; intros; simplify; equality.
+Qed.
+
+Lemma listdup_split : forall A (l : list A), firstn (length l) (l ++ l) = skipn (length l) (l ++ l).
+  repeat intros.
+  rewrite (firstn_concat l l).
+  rewrite (skipn_concat l l).
+  equality.
+Qed.
